@prefix rdf: <http://www.w3.org/1999/02/22-rdf-syntax-ns#>.
@prefix rdfs: <http://www.w3.org/2000/01/rdf-schema#> .
@prefix dbr: <http://dbpedia.org/resource/>.
@prefix owl: <http://www.w3.org/2002/07/owl#>.
@prefix foaf: <http://xmlns.com/foaf/0.1/>.
@prefix focu: <http://focu.io/schema#>.
@prefix focudata: <http://focu.io/data#>.
@prefix xsd: <http://www.w3.org/2001/XMLSchema#>.
@prefix vivo: <http://vivoweb.org/ontology/core#>.

# Classes
focu:outline
  a rdfs:Class;
  rdfs:label "Outline"@en;
  rdfs:comment "A document used to communicate important information regarding a course."@en.

focu:lecture
  a rdfs:Class;
  rdfs:label "Lecture"@en;
  rdfs:comment "An educational talk to students in a university."@en.

focu:worksheet
  a rdfs:Class;
  rdfs:label "Worksheet"@en;
  rdfs:comment "A worksheet of problems to practice offered during each lecture"@en.

focu:readings
  a rdfs:Class;
  rdfs:label "readings"@en;
  rdfs:comment "A list of readings assigned by the professor specific to a lecture"@en.

focu:reading
  a rdfs:Class;
  rdfs:label "reading"@en;
  rdfs:comment "an instance of readings assigned by the professor specific to a lecture"@en.

focu:otherMaterial
  a rdfs:Class;
  rdfs:label "Other Material"@en;
  rdfs:comment "Includes videos and images usually included in lecture slides"@en.

focu:slide
  a rdfs:Class;
  rdfs:label "Slide"@en;
  rdfs:comment "Slides are offered by the instructor during a lecture"@en.

focu:expertise
  a rdfs:Class;
  rdfs:label "Expertise"@en;
  rdfs:comment "is the set of competencies that a student is expert at (iff student passed course with better than F)"@en.

focu:completedCourse
  a rdfs:Class;
  rdfs:label "completed course"@en;
  rdfs:comment "A course completed by a student"@en.

focu:required
  a rdfs:Class;
  rdfs:label "required"@en;
  rdfs:comment "A classification of a reading"@en.

focu:supplemental
  a rdfs:Class;
  rdfs:label "supplemental"@en;
  rdfs:comment "A classification of a reading"@en.

# Properties
focu:hasExpertise
  a rdf:Property;
  rdfs:label "has expertise"@en;
  rdfs:comment "links the student to the set of expertise that he/she acquires"@en;
  rdfs:domain vivo:Student;
  rdfs:range focu:expertise.

focu:hasContent
  a rdf:Property;
  rdfs:label "has content"@en;
  rdfs:comment "Link between course and its contents"@en;
  rdfs:domain vivo:Course;
  rdfs:range focu:Lecture.

focu:hasHighestGrade
  a rdf:Property;
  rdfs:label "has highest grade"@en;
  rdfs:comment "highest grade by student at a course"@en;
  rdfs:domain focu:completedCourse;
  rdfs:range xsd:string.

focu:StudentAt
  a rdf:Property;
  rdfs:label "student at"@en;
  rdfs:comment "links the student to the university at which he/she is enrolled"@en;
  rdfs:domain vivo:Student;
  rdfs:range vivo:University.

focu:hasTaken
  a rdf:Property;
  rdfs:label "has taken"@en;
  rdfs:comment "links the student to the classes that he/she takes"@en;
  rdfs:domain vivo:Student;
  rdfs:range focu:completedCourse.

focu:refersTo
  a rdf:Property;
  rdfs:label "refers to"@en;
  rdfs:comment "links a blank node to a course. The blank node's domain is student and range is course"@en;
  rdfs:domain focu:completedCourse;
  rdfs:range vivo:Course.

# Data
